WIP: Better locales

Temporal_Plans.thy
@@ -10,12 +10,13 @@ datatype ('t :: time) upper_bound =
   LT 't |
   LE 't
 
-section \<open>State sequences and happening sequences\<close>
+section \<open>Plan validity\<close>
+text \<open>This and similar notions need to be used in multiple places. I formulate this to a 
+sufficient level of abstraction.\<close>
 
 type_synonym 'p state = "'p set"
 
-type_synonym ('p) state_sequence = "nat \<Rightarrow> ('p state)"
-
+type_synonym 'p state_sequence = "nat \<Rightarrow> ('p state)"
 
 text \<open>Invariants\<close>
 type_synonym ('p, 't) invariant_sequence = "('t \<times> 'p set) set"
@@ -24,130 +25,32 @@ text \<open>Temporal plans could be multi-sets, lists or just the range of a par
 It is only necessary that the entries do not have to be unique, because unique entries are a 
 consequence of prohibiting self-overlap. I chose a partial function.\<close>
 type_synonym ('i, 'a, 't) temp_plan = "'i \<rightharpoonup> ('a \<times> 't \<times> 't)"
-
-text \<open>This is an abstraction over a temporal planning problem\<close>
-locale temp_planning_problem =
-  fixes props::   "('proposition::linorder) set"
-    and actions:: "('action::linorder) set"
+context
+  fixes \<pi>::"('i, 'action, 'time::time) temp_plan"
     and init::    "'proposition set"
     and goal::    "'proposition set"
     and at_start::"'action  \<Rightarrow> 'snap_action"
     and at_end::  "'action  \<Rightarrow> 'snap_action"
     and over_all::"'action  \<Rightarrow> 'proposition set"
-    and lower::   "'action  \<rightharpoonup> ('time::time) lower_bound"
+    and lower::   "'action  \<rightharpoonup> 'time lower_bound"
     and upper::   "'action  \<rightharpoonup> 'time upper_bound"
     and pre::     "'snap_action \<Rightarrow> 'proposition set"
     and adds::    "'snap_action \<Rightarrow> 'proposition set"
     and dels::    "'snap_action \<Rightarrow> 'proposition set"
     and \<epsilon>::       "'time"
-  assumes wf_init:  "init \<subseteq> props" 
-      and wf_goal:  "goal \<subseteq> props"
-      and wf_acts: "let 
-          snap_props = \<lambda>s. pre s \<union> adds s \<union> dels s
-        in (\<forall>a \<in> actions. 
-          snap_props (at_start a) \<subseteq> props
-        \<and> snap_props (at_end a) \<subseteq> props
-        \<and> over_all a \<subseteq> props)"
-      and at_start_inj_on: "inj_on at_start actions"
-      and at_end_inj_on:   "inj_on at_end actions"
-      and snaps_disj:       "(at_start ` actions) \<inter> (at_end ` actions) = {}"
-      and some_props:       "card props > 0"
-      and some_actions:     "card actions > 0"
-      and finite_props:     "finite props"
-      and finite_actions:   "finite actions"
-      and eps_range:        "0 \<le> \<epsilon>"
-begin 
+begin
+text \<open>We want to define a plan in an abstract manner. This needs to be more abstract.\<close>
+definition mutex_snap_action::"'snap_action \<Rightarrow> 'snap_action \<Rightarrow> bool" where
+"mutex_snap_action a b = (
+  (pre a) \<inter> ((adds b) \<union> (dels b)) \<noteq> {} \<or>
+  ((adds a) \<inter> (dels b)) \<noteq> {} \<or>
+  (pre b) \<inter> ((adds a) \<union> (dels a)) \<noteq> {} \<or>
+  (adds b) \<inter> (dels a) \<noteq> {}
+)"
 
-text \<open>Some additional definitions\<close>
 definition apply_effects::"'proposition set \<Rightarrow> 'snap_action set \<Rightarrow> 'proposition set" where
 "apply_effects M S \<equiv> (M - \<Union>(dels ` S)) \<union> \<Union>(adds ` S)"
 
-definition mutex_snap_action::"'snap_action \<Rightarrow> 'snap_action \<Rightarrow> bool" where
-"mutex_snap_action a b = (
-  pre a \<inter> ((adds b) \<union> (dels b)) \<noteq> {} \<or>
-  (adds a \<inter> dels b) \<noteq> {} \<or>
-  pre b \<inter> ((adds a) \<union> (dels a)) \<noteq> {} \<or>
-  (adds b \<inter> dels a) \<noteq> {}
-)"
-
-lemma mutex_snap_action_symm: "mutex_snap_action a b \<longleftrightarrow> mutex_snap_action b a" 
-  unfolding mutex_snap_action_def
-  by (rule iffI) (erule disjE; blast)+
-
-abbreviation snaps::"'action \<Rightarrow> 'snap_action set" where
-"snaps a \<equiv> {at_start a, at_end a}"
-
-definition snap_actions::"'snap_action set" where
-"snap_actions \<equiv> (at_start ` actions) \<union> (at_end ` actions)"
-
-text \<open>Useful lemmas about the numberings\<close>
-
-definition "act \<equiv> (!) (sorted_list_of_set actions)"
-
-definition "p \<equiv> (!) (sorted_list_of_set props)"
-
-lemma act_bij_betw: "bij_betw act {n. n < card actions} actions"
-  unfolding act_def
-proof (rule bij_betw_nth)
-  show "distinct (sorted_list_of_set actions)" by simp
-  show "{n. n < card actions} = {..<length (sorted_list_of_set actions)}" by auto
-  show "actions = set (sorted_list_of_set actions)" using finite_actions by simp
-qed
-
-lemma act_inj_on: "inj_on act {n. n < card actions}"
-  using act_bij_betw unfolding bij_betw_def by blast
-
-lemmas act_inj_on_spec = act_inj_on[simplified inj_on_def, THEN bspec, THEN bspec, simplified mem_Collect_eq, THEN mp, rotated 2]
-
-lemma act_img_actions: "act ` {n. n < card actions} = actions"
-  using act_bij_betw unfolding bij_betw_def by blast
-
-lemma a_in_act_iff: "a \<in> actions \<longleftrightarrow> (\<exists>i < card actions. act i = a)"
-  using act_img_actions by force
-
-lemma act_pred: fixes P
-  shows "(\<forall>a \<in> actions. P a) \<longleftrightarrow> (\<forall>i < card actions. P (act i))"
-  using a_in_act_iff by auto
-
-lemma act_dom: "m < card actions \<Longrightarrow> act m \<in> actions" 
-  using act_img_actions by blast
-
-lemma p_bij_betw: "bij_betw p {n. n < card props} props"
-  unfolding p_def
-proof (rule bij_betw_nth)
-  show "distinct (sorted_list_of_set props)" by simp
-  show "{n. n < card props} = {..<length (sorted_list_of_set props)}" by auto
-  show "props = set (sorted_list_of_set props)" using finite_props by auto
-qed
-lemma p_inj_on: "inj_on p {n. n < card props}"
-  using p_bij_betw unfolding bij_betw_def by blast
-
-lemma p_img_props: "p ` {n. n < card props} = props"
-  using p_bij_betw unfolding bij_betw_def by blast
-
-lemma p_in_props_iff: "pr \<in> props \<longleftrightarrow> (\<exists>i < card props. p i = pr)"
-  using p_img_props by force
-
-lemma props_pred: fixes P
-  shows "(\<forall>pr \<in> props. P pr) \<longleftrightarrow> (\<forall>i < card props. P (p i))"
-  using p_in_props_iff by auto
-
-lemma p_dom: "n < card props \<Longrightarrow> p n \<in> props" 
-  using p_img_props by blast
-
-lemma eps_cases: 
-  assumes "\<epsilon> = 0 \<Longrightarrow> thesis"
-      and "0 \<le> \<epsilon> \<Longrightarrow> thesis"
-    shows "thesis"
-  using assms eps_range by blast
-
-subsection \<open>Temporal plans\<close>
-context
-fixes \<pi>:: "('i, 'action, 'time) temp_plan"
-begin
-
-
-text \<open>Happening Time Points\<close>
 definition htps::"'time set" where
 "htps \<equiv> {t |a t d. (a, t, d) \<in> ran \<pi>} \<union> {t + d |a t d. (a, t, d) \<in> ran \<pi>}"
 
@@ -225,7 +128,136 @@ definition valid_state_sequence::"'proposition state_sequence \<Rightarrow> bool
         \<and> pres \<subseteq> (M i)))
 )"
 
-text \<open>For the definition of a valid plan\<close>
+definition satisfies_duration_bounds::"'action \<Rightarrow> 'time \<Rightarrow> bool" where
+"satisfies_duration_bounds a t \<equiv> 
+  let lb = (case (lower a) of 
+    Some (GT t') \<Rightarrow> t' < t
+  | Some (GE t') \<Rightarrow> t' \<le> t
+  | None \<Rightarrow> True);
+  ub = (case (upper a) of 
+    Some (LT t') \<Rightarrow> t < t'
+  | Some (LE t') \<Rightarrow> t \<le> t'
+  | None \<Rightarrow> True)
+  in lb \<and> ub
+"
+(* An action with a duration of 0 is an instant snap-action. We restrict this to 0 < d for some 
+proofs, because of how some automata are constructed. *)
+definition durations_ge_0::bool where
+"durations_ge_0 \<equiv> \<forall>a t d. (a, t, d) \<in> ran \<pi> \<longrightarrow> 0 \<le> d"
+
+definition durations_valid::bool where
+"durations_valid \<equiv> \<forall>a t d. (a, t, d) \<in> ran \<pi> \<longrightarrow> satisfies_duration_bounds a d"
+
+definition valid_plan::"bool" where
+"valid_plan \<equiv> \<exists>M. 
+    valid_state_sequence M
+    \<and> M 0 = init
+    \<and> goal \<subseteq> M (length htpl)
+    \<and> durations_ge_0
+    \<and> durations_valid
+    \<and> nm_happ_seq plan_happ_seq"
+end
+
+text \<open>By making the planning domain finite, it becomes possible to reduce it to a timed automaton
+with a finite number of states.\<close>
+locale temp_planning_problem =
+  fixes props::   "('proposition::linorder) set"
+    and actions:: "('action::linorder) set"
+    and init::    "'proposition set"
+    and goal::    "'proposition set"
+    and at_start::"'action  \<Rightarrow> 'snap_action"
+    and at_end::  "'action  \<Rightarrow> 'snap_action"
+    and over_all::"'action  \<Rightarrow> 'proposition set"
+    and lower::   "'action  \<rightharpoonup> ('time::time) lower_bound"
+    and upper::   "'action  \<rightharpoonup> 'time upper_bound"
+    and pre::     "'snap_action \<Rightarrow> 'proposition set"
+    and adds::    "'snap_action \<Rightarrow> 'proposition set"
+    and dels::    "'snap_action \<Rightarrow> 'proposition set"
+    and \<epsilon>::       "'time"
+  assumes wf_init:  "init \<subseteq> props" 
+      and wf_goal:  "goal \<subseteq> props"
+      and at_start_inj_on: "inj_on at_start actions"
+      and at_end_inj_on:   "inj_on at_end actions"
+      and snaps_disj:       "(at_start ` actions) \<inter> (at_end ` actions) = {}"
+      and some_props:       "card props > 0"
+      and some_actions:     "card actions > 0"
+      and finite_props:     "finite props"
+      and finite_actions:   "finite actions"
+      and eps_range:        "0 \<le> \<epsilon>"
+begin 
+
+
+abbreviation snaps::"'action \<Rightarrow> 'snap_action set" where
+"snaps a \<equiv> {at_start a, at_end a}"
+
+definition snap_actions::"'snap_action set" where
+"snap_actions \<equiv> (at_start ` actions) \<union> (at_end ` actions)"
+
+text \<open>Useful lemmas about the numberings\<close>
+
+definition "act \<equiv> (!) (sorted_list_of_set actions)"
+
+definition "p \<equiv> (!) (sorted_list_of_set props)"
+
+lemma act_bij_betw: "bij_betw act {n. n < card actions} actions"
+  unfolding act_def
+proof (rule bij_betw_nth)
+  show "distinct (sorted_list_of_set actions)" by simp
+  show "{n. n < card actions} = {..<length (sorted_list_of_set actions)}" by auto
+  show "actions = set (sorted_list_of_set actions)" using finite_actions by simp
+qed
+
+lemma act_inj_on: "inj_on act {n. n < card actions}"
+  using act_bij_betw unfolding bij_betw_def by blast
+
+lemmas act_inj_on_spec = act_inj_on[simplified inj_on_def, THEN bspec, THEN bspec, simplified mem_Collect_eq, THEN mp, rotated 2]
+
+lemma act_img_actions: "act ` {n. n < card actions} = actions"
+  using act_bij_betw unfolding bij_betw_def by blast
+
+lemma a_in_act_iff: "a \<in> actions \<longleftrightarrow> (\<exists>i < card actions. act i = a)"
+  using act_img_actions by force
+
+lemma act_pred: fixes P
+  shows "(\<forall>a \<in> actions. P a) \<longleftrightarrow> (\<forall>i < card actions. P (act i))"
+  using a_in_act_iff by auto
+
+lemma act_dom: "m < card actions \<Longrightarrow> act m \<in> actions" 
+  using act_img_actions by blast
+
+lemma p_bij_betw: "bij_betw p {n. n < card props} props"
+  unfolding p_def
+proof (rule bij_betw_nth)
+  show "distinct (sorted_list_of_set props)" by simp
+  show "{n. n < card props} = {..<length (sorted_list_of_set props)}" by auto
+  show "props = set (sorted_list_of_set props)" using finite_props by auto
+qed
+lemma p_inj_on: "inj_on p {n. n < card props}"
+  using p_bij_betw unfolding bij_betw_def by blast
+
+lemma p_img_props: "p ` {n. n < card props} = props"
+  using p_bij_betw unfolding bij_betw_def by blast
+
+lemma p_in_props_iff: "pr \<in> props \<longleftrightarrow> (\<exists>i < card props. p i = pr)"
+  using p_img_props by force
+
+lemma props_pred: fixes P
+  shows "(\<forall>pr \<in> props. P pr) \<longleftrightarrow> (\<forall>i < card props. P (p i))"
+  using p_in_props_iff by auto
+
+lemma p_dom: "n < card props \<Longrightarrow> p n \<in> props" 
+  using p_img_props by blast
+
+lemma eps_cases: 
+  assumes "\<epsilon> = 0 \<Longrightarrow> thesis"
+      and "0 \<le> \<epsilon> \<Longrightarrow> thesis"
+    shows "thesis"
+  using assms eps_range by blast
+
+subsection \<open>Temporal plans\<close>
+context
+fixes \<pi>:: "('i, 'action, 'time) temp_plan"
+begin
 
 definition no_self_overlap::"bool" where
 "no_self_overlap \<equiv> \<not>(\<exists>i j a t d u e. i \<noteq> j
@@ -249,57 +281,27 @@ lemma no_self_overlap_spec:
 definition plan_actions_in_problem::bool where
 "plan_actions_in_problem \<equiv> \<forall>a t d. (a, t, d) \<in> ran \<pi> \<longrightarrow> a \<in> actions"
 
-
-definition satisfies_duration_bounds::"'action \<Rightarrow> 'time \<Rightarrow> bool" where
-"satisfies_duration_bounds a t \<equiv> 
-  let lb = (case (lower a) of 
-    Some (GT t') \<Rightarrow> t' < t
-  | Some (GE t') \<Rightarrow> t' \<le> t
-  | None \<Rightarrow> True);
-  ub = (case (upper a) of 
-    Some (LT t') \<Rightarrow> t < t'
-  | Some (LE t') \<Rightarrow> t \<le> t'
-  | None \<Rightarrow> True)
-  in lb \<and> ub
-"
-
 definition durations_positive::bool where
 "durations_positive \<equiv> \<forall>a t d. (a, t, d) \<in> ran \<pi> \<longrightarrow> 0 < d"
-
-definition durations_valid::bool where
-"durations_valid \<equiv> \<forall>a t d. (a, t, d) \<in> ran \<pi> \<longrightarrow> satisfies_duration_bounds a d"
-
-definition valid_plan::"bool" where
-"valid_plan \<equiv> \<exists>M. 
-    valid_state_sequence M
-    \<and> no_self_overlap
-    \<and> M 0 = init
-    \<and> goal \<subseteq> M (length htpl)
-    \<and> plan_actions_in_problem
-    \<and> durations_positive
-    \<and> durations_valid
-    \<and> nm_happ_seq plan_happ_seq"
-
 
 definition finite_plan::bool where
 "finite_plan \<equiv> finite (dom \<pi>)"
 
-lemma a_in_B_iff_t_in_htps: "(\<exists>a. a \<in> happ_at plan_happ_seq t) \<longleftrightarrow> (t \<in> htps)"
+lemma a_in_B_iff_t_in_htps: "(\<exists>a. a \<in> happ_at (plan_happ_seq \<pi> at_start at_end) t) \<longleftrightarrow> (t \<in> htps \<pi>)"
 proof
-  assume "\<exists>a. a \<in> happ_at plan_happ_seq t"
+  assume "\<exists>a. a \<in> happ_at (plan_happ_seq \<pi> at_start at_end) t"
   then obtain a where
-    "(t, a) \<in> plan_happ_seq" using happ_at_def by auto
-  thus "t \<in> htps" using plan_happ_seq_def htps_def by auto
+    "(t, a) \<in> plan_happ_seq \<pi> at_start at_end" unfolding happ_at_def plan_happ_seq_def by fast
+  thus "t \<in> htps \<pi>" unfolding plan_happ_seq_def htps_def by blast
 next
-  assume "t \<in> local.htps"
+  assume "t \<in> htps \<pi>"
   then obtain a where
-    "(t, a) \<in> plan_happ_seq" using plan_happ_seq_def htps_def by force
-  thus "\<exists>a. a \<in> happ_at plan_happ_seq t" using happ_at_def by blast
+    "(t, a) \<in> plan_happ_seq \<pi> at_start at_end" unfolding plan_happ_seq_def htps_def by force
+  thus "\<exists>a. a \<in> happ_at (plan_happ_seq \<pi> at_start at_end) t" unfolding happ_at_def by blast
 qed
 
-
 lemma at_start_in_happ_seqE: 
-  assumes in_happ_seq: "(t, at_start a) \<in> plan_happ_seq"
+  assumes in_happ_seq: "(t, at_start a) \<in> plan_happ_seq \<pi> at_start at_end"
       and a_in_actions: "a \<in> actions"
       and no_self_overlap
       and durations_positive
@@ -363,7 +365,7 @@ proof -
 qed
 
 lemma at_end_in_happ_seqE:
-  assumes in_happ_seq: "(s, at_end a) \<in> plan_happ_seq"
+  assumes in_happ_seq: "(s, at_end a) \<in> plan_happ_seq \<pi> at_start at_end"
       and a_in_actions: "a \<in> actions"
       and no_self_overlap
       and durations_positive
@@ -437,14 +439,14 @@ proof -
 qed
 
 lemma in_happ_seqE:
-  assumes in_happ_seq: "(t, snap) \<in> plan_happ_seq"
+  assumes in_happ_seq: "(t, snap) \<in> plan_happ_seq \<pi> at_start at_end"
   shows "\<exists>t d a. (a, t, d) \<in> ran \<pi> \<and> (at_start a = snap \<or> at_end a = snap)"
   using assms unfolding plan_happ_seq_def by blast
 
 
 lemma finite_htps: 
   assumes "finite_plan"
-    shows "finite htps"
+    shows "finite (htps \<pi>)"
 proof -
   have 1: "finite ((\<lambda>(a, t, d). t) ` (ran \<pi>))" 
     "finite ((\<lambda>(a, t, d). t + d) ` (ran \<pi>))"
@@ -455,36 +457,34 @@ proof -
   moreover
   have " (\<lambda>(a, t, d). t + d) ` (ran \<pi>)  = {t + d |a t d. (a, t, d) \<in> ran \<pi>}" by force
   ultimately
-  show "finite htps" unfolding htps_def by auto
+  show "finite (htps \<pi>)" unfolding htps_def by auto
 qed
-
-find_theorems "sorted_key_list_of_set ?f ?A"
 
 lemma set_htpl_eq_htps: 
   assumes finite_plan
-  shows "htps = set htpl" 
+  shows "htps \<pi> = set (htpl \<pi>)" 
   unfolding htpl_def set_sorted_list_of_set[OF finite_htps[OF assms(1)]]
   by blast
 
 
-lemma time_index_bij_betw_list: "bij_betw time_index {n. n < length htpl} (set htpl)"
+lemma time_index_bij_betw_list: "bij_betw (time_index \<pi>) {n. n < length (htpl \<pi>)} (set (htpl \<pi>))"
   using bij_betw_nth distinct_sorted_list_of_set htpl_def[symmetric] lessThan_def
   by metis
 
-lemma time_index_inj_on_list: "inj_on time_index {n. n < length htpl}" 
+lemma time_index_inj_on_list: "inj_on (time_index \<pi>) {n. n < length (htpl \<pi>)}" 
   using bij_betw_def time_index_bij_betw_list by blast
 
-lemma time_index_img_list: "time_index ` {n. n < length htpl} = set htpl"
+lemma time_index_img_list: "(time_index \<pi>) ` {n. n < length (htpl \<pi>)} = set (htpl \<pi>)"
   using time_index_bij_betw_list unfolding bij_betw_def by blast
 
-lemma card_htps_len_htpl: "card htps = length htpl" using htpl_def by simp
+lemma card_htps_len_htpl: "card (htps \<pi>) = length (htpl \<pi>)" unfolding htpl_def by simp
 
 lemma time_index_bij_betw_set:
   assumes "finite_plan"
-  shows "bij_betw time_index {n. n < card htps} htps"
+  shows "bij_betw (time_index \<pi>) {n. n < card (htps \<pi>)} (htps \<pi>)"
 proof -
-  have 3: "distinct htpl" unfolding htpl_def by simp
-  show "bij_betw time_index {n. n < card htps} htps"
+  have 3: "distinct (htpl \<pi>)" unfolding htpl_def by simp
+  show "bij_betw (time_index \<pi>) {n. n < card (htps \<pi>)} (htps \<pi>)"
     apply (subst card_htps_len_htpl)
     apply (subst set_htpl_eq_htps[OF assms])
     using time_index_bij_betw_list
@@ -493,54 +493,47 @@ qed
 
 lemma time_index_inj_on_set:
   assumes "finite_plan"
-  shows "inj_on time_index {n. n < card htps}" 
+  shows "inj_on (time_index \<pi>) {n. n < card (htps \<pi>)}" 
   using time_index_bij_betw_set[OF assms] bij_betw_def by blast
 
 lemma time_index_img_set:
   assumes "finite_plan"
-  shows "time_index ` {n. n < card htps} = htps" 
+  shows "(time_index \<pi>) ` {n. n < card (htps \<pi>)} = (htps \<pi>)" 
   using time_index_bij_betw_set[OF assms] unfolding bij_betw_def by blast
 
-
-find_theorems name: "key*list*of*set"
-
-thm strict_sorted_list_of_set
-
-find_theorems name: "sorted*nth"
-
-lemmas time_index_strict_sorted_list = strict_sorted_list_of_set[of htps, simplified htpl_def[symmetric], THEN sorted_wrt_nth_less]
+lemmas time_index_strict_sorted_list = strict_sorted_list_of_set[of \<open>htps \<pi>\<close>, simplified htpl_def[symmetric], THEN sorted_wrt_nth_less]
 
 lemma time_index_strict_mono_on_list: 
-  "strict_mono_on {n. n < length htpl} time_index" 
+  "strict_mono_on {n. n < length (htpl \<pi>)} (time_index \<pi>)" 
   using time_index_strict_sorted_list unfolding monotone_on_def
   by blast
 
-lemmas time_index_sorted_list = sorted_list_of_set(2)[of htps, simplified htpl_def[symmetric], THEN sorted_nth_mono]
+lemmas time_index_sorted_list = sorted_list_of_set(2)[of \<open>htps \<pi>\<close>, simplified htpl_def[symmetric], THEN sorted_nth_mono]
 
 lemma time_index_strict_sorted_list':
-  assumes i: "i < length htpl"
-      and ti: "time_index i < time_index j"
+  assumes i: "i < length (htpl \<pi>)"
+      and ti: "time_index \<pi> i < time_index \<pi> j"
     shows "i < j"
 proof (rule ccontr)
   assume "\<not> i < j"
   hence "j \<le> i" by simp
-  hence "time_index j \<le> time_index i" using i time_index_sorted_list by simp
+  hence "time_index \<pi> j \<le> time_index \<pi> i" using i time_index_sorted_list by simp
   thus False using ti by simp
 qed
 
 lemma time_index_sorted_list':
-  assumes i: "i < length htpl"
-      and ti: "time_index i \<le> time_index j"
+  assumes i: "i < length (htpl \<pi>)"
+      and ti: "time_index \<pi> i \<le> time_index \<pi> j"
     shows "i \<le> j"
 proof (rule ccontr)
   assume "\<not> i \<le> j"
   hence "j < i" by simp
-  hence "time_index j < time_index i" using i time_index_strict_sorted_list by simp
+  hence "time_index \<pi> j < time_index \<pi> i" using i time_index_strict_sorted_list by simp
   thus False using ti by simp
 qed
 
 lemma time_index_mono_on_list:
-  "mono_on {n. n < length htpl} time_index" 
+  "mono_on {n. n < length (htpl \<pi>)} (time_index \<pi>)" 
   using time_index_sorted_list unfolding monotone_on_def by auto
 
 lemmas time_index_strict_sorted_set = time_index_strict_sorted_list[simplified card_htps_len_htpl[symmetric]]
@@ -552,15 +545,15 @@ lemmas time_index_sorted = time_index_sorted_list time_index_sorted_set time_ind
   time_index_sorted_list' time_index_sorted_set' time_index_strict_sorted_list' time_index_strict_sorted_set'
 
 lemma no_non_indexed_time_points: 
-  assumes a: "(Suc l) < length htpl"
-  shows "\<not> (\<exists>t'. (time_index l) < t' \<and> t' < (time_index (Suc l)) \<and> t' \<in> set htpl)"
+  assumes a: "(Suc l) < length (htpl \<pi>)"
+  shows "\<not> (\<exists>t'. (time_index \<pi> l) < t' \<and> t' < (time_index \<pi> (Suc l)) \<and> t' \<in> set (htpl \<pi>))"
 proof (rule notI)
-  assume "\<exists>t'>time_index l. t' < time_index (Suc l) \<and> t' \<in> set htpl"
+  assume "\<exists>t'>time_index \<pi> l. t' < time_index \<pi> (Suc l) \<and> t' \<in> set (htpl \<pi>)"
   with time_index_bij_betw_list
   obtain l' where
-    l': "l' < length htpl"
-    "time_index l < time_index l'"
-    "time_index l' < time_index (Suc l)"
+    l': "l' < length (htpl \<pi>)"
+    "time_index \<pi> l < time_index \<pi> l'"
+    "time_index \<pi> l' < time_index \<pi> (Suc l)"
     by (metis in_set_conv_nth)
   
   have "l' < (Suc l)" using l'(1, 3) time_index_strict_sorted_list' by simp
@@ -572,12 +565,131 @@ qed
 
 lemma no_actions_between_indexed_timepoints: 
   assumes "finite_plan"
-    "(Suc l) < length htpl"
-  shows "\<not> (\<exists>t'>time_index l. t' < time_index (Suc l) \<and> a \<in> happ_at plan_happ_seq t')"
+    "(Suc l) < length (htpl \<pi>)"
+  shows "\<not> (\<exists>t'>time_index \<pi> l. t' < time_index \<pi> (Suc l) \<and> a \<in> happ_at (plan_happ_seq \<pi> at_start at_end) t')"
   using no_non_indexed_time_points[OF assms(2)] 
-    a_in_B_iff_t_in_htps finite_htps[OF assms(1)] htpl_def by auto
+    a_in_B_iff_t_in_htps finite_htps[OF assms(1)] 
+  unfolding htpl_def by auto
+
+text \<open>This is a property of plan actions\<close>
+definition wf_act where
+"wf_act a \<equiv> let snap_props = \<lambda>s. pre s \<union> adds s \<union> dels s
+  in (
+    snap_props (at_start a) \<subseteq> props
+  \<and> snap_props (at_end a) \<subseteq> props
+  \<and> over_all a \<subseteq> props)" 
+
+definition wf_acts where
+"wf_acts \<equiv> (\<forall>(a, t, d) \<in> ran \<pi>. wf_act a)"
 
 end
 end
 
+datatype (act: 'a) snap_action = 
+  AtStart 'a |
+  AtEnd 'a
+locale finite_domain_planning =
+  fixes props::   "('proposition::linorder) set"
+    and acts::    "('action::linorder) set"
+    and init::    "'proposition set"
+    and goal::    "'proposition set"
+    and at_start::"'action  \<Rightarrow> 'snap_action"
+    and at_end::  "'action  \<Rightarrow> 'snap_action"
+    and over_all::"'action  \<Rightarrow> 'proposition set"
+    and lower::   "'action  \<rightharpoonup> ('time::time) lower_bound"
+    and upper::   "'action  \<rightharpoonup> 'time upper_bound"
+    and pre::     "'snap_action \<Rightarrow> 'proposition set"
+    and adds::    "'snap_action \<Rightarrow> 'proposition set"
+    and dels::    "'snap_action \<Rightarrow> 'proposition set"
+    and \<epsilon>::       "'time"
+  assumes some_props:       "card props > 0"
+      and some_actions:     "card acts > 0"
+      and finite_props:     "finite props"
+      and finite_actions:   "finite acts"
+      and eps_range:        "0 \<le> \<epsilon>"
+begin
+
+  definition "init_imp = init \<inter> props"
+  definition "goal_imp = goal \<inter> props"
+  
+  fun app_snap::"('snap_action \<Rightarrow> 'proposition set) \<Rightarrow> 'action snap_action \<Rightarrow> 'proposition set" where
+  "app_snap f (AtStart a) = f (at_start a)" |
+  "app_snap f (AtEnd a) = f (at_end a)"
+  
+  definition pre_imp::"'action snap_action \<Rightarrow> 'proposition set" where
+  "pre_imp = (\<inter>) props o app_snap pre"
+  
+  definition add_imp::"'action snap_action \<Rightarrow> 'proposition set" where
+  "add_imp = app_snap adds"
+  
+  definition del_imp::"'action snap_action \<Rightarrow> 'proposition set" where
+  "del_imp = app_snap dels"
+
+  definition over_all_imp::"'action \<Rightarrow> 'proposition set" where
+  "over_all_imp = (\<inter>) props o over_all"
+
+  sublocale temp_planning_problem props acts init_imp goal_imp AtStart AtEnd over_all_imp lower upper pre_imp add_imp del_imp \<epsilon>
+  proof
+    show "init_imp \<subseteq> props" "goal_imp \<subseteq> props" unfolding init_imp_def goal_imp_def by simp+
+    show "inj_on AtStart acts" "inj_on AtEnd acts" unfolding inj_on_def by blast+
+    show "AtStart ` acts \<inter> AtEnd ` acts = {}" by blast
+    show "0 < card props" by (rule some_props)
+    show "0 < card acts" by (rule some_actions)
+    show "finite props" by (rule finite_props)
+    show "finite acts" by (rule finite_actions)
+    show "0 \<le> \<epsilon>" by (rule eps_range)
+  qed 
+
+  context 
+    fixes \<pi>::"('i, 'action, 'time) temp_plan"
+  begin
+    (* PDDL plans must not modify equalities, but can use them in preconditions. *)
+    definition act_mod_props where
+      "act_mod_props a \<equiv> (
+        let snap_effs = (\<lambda>s. adds s \<union> dels s)
+        in snap_effs (at_start a) \<subseteq> props \<and> snap_effs (at_end a) \<subseteq> props
+       )"
+  
+    definition plan_acts_mod_props where
+      "plan_acts_mod_props = (\<forall>(a, t, d) \<in> ran \<pi>. act_mod_props a)"
+
+    definition act_prec_ran where
+      "act_prec_ran a \<equiv> (
+        over_all a \<subseteq> props \<union> init
+      \<and> pre (at_start a) \<subseteq> props \<union> init
+      \<and> pre (at_end a) \<subseteq> props \<union> init
+      )"
+
+    definition plan_acts_prec_ranges where
+      "plan_acts_prec_ranges \<equiv> (\<forall>(a, t, d) \<in> ran \<pi>. act_prec_ran a)"
+
+    definition restr_props_in_state_seq::"'proposition state_sequence \<Rightarrow> 'proposition state_sequence" where
+      "restr_props_in_state_seq M i \<equiv> (M i \<inter> props)"
+    
+    context 
+      assumes prec_rans: plan_acts_prec_ranges
+          and prop_upds: plan_acts_mod_props
+    begin
+      lemma over_all_imp_eq: "(\<lambda>t. invs_at (plan_inv_seq \<pi> over_all) t \<inter> props) = invs_at (plan_inv_seq \<pi> over_all_imp)"
+        by (rule ext; auto simp: plan_inv_seq_def over_all_imp_def invs_at_def)
+
+    lemma happ_seq_imp_eq: "adds ` (happ_at (plan_happ_seq \<pi> at_start at_end) t) = add_imp ` (happ_at (plan_happ_seq \<pi> AtStart AtEnd) t)"
+    proof (rule equalityI; rule subsetI)
+      fix x
+      assume "x \<in> adds ` happ_at (plan_happ_seq \<pi> at_start at_end) t"
+      show "x \<in> add_imp ` happ_at (plan_happ_seq \<pi> AtStart AtEnd) t" sorry
+    qed
+
+      lemma valid_state_seq_eq: "valid_state_sequence \<pi> at_start at_end over_all pre adds dels M =
+        valid_state_sequence \<pi> AtStart AtEnd over_all_imp pre_imp add_imp del_imp (restr_props_in_state_seq M)"
+        unfolding valid_state_sequence_def
+        sorry
+
+      lemma plan_with_eq_is_plan_without_eq: "valid_plan \<pi> init goal at_start at_end over_all lower upper pre adds dels \<epsilon>
+              \<equiv> valid_plan \<pi> init_imp goal_imp AtStart AtEnd over_all_imp lower upper pre_imp add_imp del_imp \<epsilon>"
+        sorry
+    end
+
+  end
+end
 end
